intermediate

theories/FRACTRAN/Utils/FRACTRAN_computable.v
@@ -1,30 +1,39 @@
 Require Import Undecidability.FRACTRAN.FRACTRAN.
 
-From Coq Require Import List Vector Nat.
+From Coq Require Import List Vector Nat Arith Lia.
+From Undecidability.FRACTRAN Require Import prime_seq.
 Import ListNotations Vector.VectorNotations.
-From Undecidability Require Import Utils.prime FRACTRAN_sss Code.sss fractran_utils.
+From Undecidability Require Import Utils.gcd Utils.prime FRACTRAN_sss Code.sss fractran_utils.
 
-Fixpoint enc {k} p i (v : Vector.t nat k) : nat := 
+Fixpoint enc {k} i (v : Vector.t nat k) : nat := 
   match v with
   | @nil _ => 1
-  | x :: v => (p i) ^ x * enc p (S i) v
+  | x :: v => (qs i) ^ x * enc (S i) v
   end.
 
-Definition FRACTRAN_computable {k} (p : nat -> nat) (R : Vector.t nat k -> nat -> Prop) := 
+Definition FRACTRAN_computable {k} (R : Vector.t nat k -> nat -> Prop) := 
   exists P : list (nat * nat), fractran_regular P /\
     forall v : Vector.t nat k,
-      (forall m, R v m <-> fractran_eval P (enc p 1 v) ((p 0)^m))
-    /\ (forall n, fractran_eval P (enc p 1 v) n -> exists m, n = (p 0) ^ m).
-
-Lemma FRACTRAN_computable_functional {k} (p : nat -> nat) (R : Vector.t nat k -> nat -> Prop) :
-  (forall i j, p i = p j -> i = j) ->
-  (forall i, prime (p i)) ->
-  FRACTRAN_computable p R -> forall v m1 m2, R v m1 -> R v m2 -> m1 = m2.
+      (forall m, R v m <-> exists j, fractran_eval P (ps 1 * enc 2 v) (j * (qs 1)^m) /\ ~ divides (qs 1) j).
+      
+Lemma FRACTRAN_computable_functional {k} (R : Vector.t nat k -> nat -> Prop) :
+  FRACTRAN_computable R -> forall v m1 m2, R v m1 -> R v m2 -> m1 = m2.
 Proof.
-  intros Hpf Hpp (P & Hreg & HP) v m1 m2 H1 % HP H2 % HP. 
+  intros (P & Hreg & HP) v m1 m2 (j1 & k1 & v1 & H1) % HP (j2 & k2 & v2 & H2) % HP. 
   eapply eval_iff in H1 as [H1 H1'], H2 as [H2 H2'].
-  assert (p 0 ^ m1 = p 0 ^ m2).
-  - eapply fractran_compute_fun; eauto.
-  - assert (prime (p 0)) as ? % prime_ge_2 by eauto.
-    eapply PeanoNat.Nat.pow_inj_r; try eassumption.
+  eapply fractran_compute_fun in H1'; eauto.
+  eapply power_factor_uniq with (x := ps j1 * enc 2 v1) (y := ps j2 * enc 2 v2) (p := qs 1).
+  - epose proof (nxtprime_spec1 (nxtprime (nxtprime 2))). cbn. lia.
+  - intros [[] % qs_ps_div | H] % prime_div_mult.
+    + change (enc 1 v1) with (exp 1 v1) in H.
+      eapply qs_exp_div in H; lia.
+    + eapply nxtprime_spec2.
+  - intros [[] % qs_ps_div | H] % prime_div_mult.
+    + clear - H. induction v2.
+      * eapply divides_1_inv in H. cbn in H.
+        pose proof (nxtprime_spec2 (nxtprime (nxtprime 2))).
+        eapply prime_ge_2 in H0. lia.
+      * eapply qs_exp_div in H; lia.
+    + eapply nxtprime_spec2.
+  - lia.
 Qed.
