theories/MinskyMachines/Util/MM_computable.v
@@ -4,7 +4,7 @@ From Coq Require Import List Vector.
 Import ListNotations Vector.VectorNotations.
 
 Definition MM_computable {k} (R : Vector.t nat k -> nat -> Prop) := 
-  exists n : nat, exists i : nat, exists P : list (mm_instr (Fin.t (1 + k + n))),
+  exists n : nat, exists P : list (mm_instr (Fin.t (1 + k + n))),
     forall v : Vector.t nat k,
       (forall m, R v m <->
-         exists c v', @MM.eval (1 + k + n) (i, P) (i, (0 :: v) ++ Vector.const 0 n) (c, m :: v')).
+         exists c v', @MM.eval (1 + k + n) (1, P) (1, (0 :: v) ++ Vector.const 0 n) (c, m :: v')).
