theories/FRACTRAN/Reductions/MM_computable_to_FRACTRAN_computable.v
@@ -1,0 +1,25 @@
+From Undecidability.MinskyMachines Require Import MM_computable MM_sss.
+From Undecidability.FRACTRAN Require Import FRACTRAN_computable mm_fractran prime_seq.
+
+Opaque ps qs.
+
+Theorem MM_computable_to_FRACTRAN_computable {k} (R : Vector.t nat k -> nat -> Prop) :
+  MM_computable R -> FRACTRAN_computable R.
+Proof.
+  intros (n & P & H). setoid_rewrite eval_iff in H.
+  pose proof (mm_fractran_n_strong P) as (P' & regP & HP).
+  exists P'. setoid_rewrite H. clear H. split. 1: eapply regP.
+  setoid_rewrite FRACTRAN_sss.eval_iff. fold plus.
+  intros v. split. 1: intros m; split.
+  - fold plus in *. intros (j & v' & H).
+    edestruct HP as [[j' Hj'] _].
+    + eexists. eapply H.
+    + rewrite FRACTRAN_sss.eval_iff in Hj'.
+      exists j'. eexists. exists v'. change (@enc (k + n)) with (@exp (k + n)). 
+      eexists. eexists. unfold encode_state in Hj'. cbn in *.
+      rewrite !PeanoNat.Nat.add_0_r in *.
+      admit. admit.
+  - intros (j & k' & v' & H1 & H2). 
+    admit.
+  - admit.
+Admitted.
